Factored out MR goal

proof/correctness/avx2/MLKEM_InnerPKE_avx2.ec
@@ -839,6 +839,7 @@ move => *; rewrite /signed_bound_cxq /b16 qE /#.
 qed.
 
 import InnerPKE.
+
 lemma mlkem_correct_kg_avx2 mem _pkp _skp  : 
    equiv [Jkem_avx2.M(Jkem_avx2.Syscall).__indcpa_keypair ~ InnerPKE.kg_derand : 
        Glob.mem{1} = mem /\ to_uint pkp{1} = _pkp /\ to_uint skp{1} = _skp /\ 
@@ -1266,6 +1267,189 @@ qed.
 
 (***************************************************)
 
+require import WArray1088 WArray1536 Array4.
+
+module AuxPolyVecCompress10 = {
+    proc avx2_orig(ctp : W64.t, bp : W16.t Array768.t) : WArray1088.t = {
+       bp <@  Jkem_avx2.M(Jkem_avx2.Syscall).__polyvec_reduce_sig(bp);  
+       Jkem_avx2.M(Jkem_avx2.Syscall).__polyvec_compress(ctp, bp);
+       return witness;
+    }
+
+proc __polyvec_compress_avx2(a : W16.t Array768.t) : WArray1088.t = {
+    var aux : int;
+    var b0 : W256.t;
+    var b1 : W256.t;
+    var b2 : W256.t;
+    var mask10 : W256.t;
+    var shift : W256.t;
+    var sllv_indx : W256.t;
+    var shuffle : W256.t;
+    var i : int;
+    var a0 : W256.t;
+    var lo : W128.t;
+    var hi : W128.t;
+    var rr : WArray1088.t <- witness;
+    
+    b0 <- VPBROADCAST_16u16 compress10_b0;
+    b1 <- VPBROADCAST_16u16 compress10_b1;
+    b2 <- VPBROADCAST_16u16 pc_shift1_s;
+    mask10 <- VPBROADCAST_16u16 pvc_mask_s;
+    shift <- VPBROADCAST_8u32 compress10_shift;
+    sllv_indx <- VPBROADCAST_4u64 pvc_sllvdidx_s;
+    shuffle <- get256 ((init8 (fun (i_0 : int) => pvc_shufbidx_s.[i_0])))%WArray32 0;
+    aux <- 3 * 256 %/ 16;
+    i <- 0;
+    while (i < aux){
+      a0 <- (get256 ((WArray1536.init16 (fun (i_0 : int) => a.[i_0]))) i);
+      a0 <@ Jkem_avx2.M(Syscall).compress10_16x16_inline(a0, b0, b1, b2, mask10);
+      (lo, hi) <@ Jkem_avx2.M(Syscall).pack10_16x16(a0, shift, sllv_indx, shuffle);
+      rr <- WArray1088.set128_direct rr (i*20+0) lo;
+      rr <- WArray1088.set32_direct rr (i*20+16) (VPEXTR_32 hi W8.zero);
+(* 
+      Glob.mem <- storeW128 Glob.mem (to_uint (r + (of_int (i * 20 + 0))%W64)) lo;
+      Glob.mem <- storeW32 Glob.mem (to_uint (r + (of_int (i * 20 + 16))%W64)) (VPEXTR_32 hi W8.zero);
+*)
+      i <- i + 1;
+    }
+    
+    return rr;
+  }
+
+    proc avx2(bp : W16.t Array768.t) : WArray1088.t = {
+       var rr : WArray1088.t;
+       bp <@  Jkem_avx2.M(Jkem_avx2.Syscall).__polyvec_reduce_sig(bp);  
+       rr <@ __polyvec_compress_avx2(bp);
+       return rr;
+    }
+
+    proc ref_orig(ctp : W64.t, bp : W16.t Array768.t)  : WArray1088.t = {
+       bp <@ Jkem.M(Syscall).__polyvec_reduce(bp); 
+       Jkem.M(Syscall).__polyvec_compress(ctp, bp);
+       return witness;
+    }
+
+proc __polyvec_compress_ref(a : W16.t Array768.t) : WArray1088.t = {
+    var aux : int;
+    var i : int;
+    var j : int;
+    var aa : W16.t Array768.t;
+    var k : int;
+    var t : W64.t Array4.t;
+    var c : W16.t;
+    var b : W16.t;
+    var rr : WArray1088.t <- witness;
+    
+    aa <- witness;
+    t <- witness;
+    i <- 0;
+    j <- 0;
+    aa <@ M(Syscall).__polyvec_csubq(a);
+    while (i < (3 * 256 - 3)){
+      k <- 0;
+      while (k < 4){
+        t.[k] <- zeroextu64 aa.[i];
+        i <- i + 1;
+        t.[k] <- (t.[k]) `<<` (of_int 10)%W8;
+        t.[k] <- (t.[k]) + (of_int 1665)%W64;
+        t.[k] <- (t.[k]) * (of_int 1290167)%W64;
+        t.[k] <- (t.[k]) `>>` (of_int 32)%W8;
+        t.[k] <- (t.[k]) `&` (of_int 1023)%W64;
+        k <- k + 1;
+      }
+      c <- truncateu16 (t.[0]);
+      c <- c `&` (of_int 255)%W16;
+      rr.[j] <- (truncateu8 c);
+      (* 
+      Glob.mem <- storeW8 Glob.mem (to_uint (rp + j)) (truncateu8 c); 
+      *)
+      j <- j + 1;
+      b <- truncateu16 (t.[0]);
+      b <- b `>>` (of_int 8)%W8;
+      c <- truncateu16 (t.[1]);
+      c <- c `<<` (of_int 2)%W8;
+      c <- c `|` b;
+      rr.[j] <- (truncateu8 c);
+      (* 
+      Glob.mem <- storeW8 Glob.mem (to_uint (rp + j)) (truncateu8 c); 
+      *)
+      j <- j + 1;
+      b <- truncateu16 (t.[1]);
+      b <- b `>>` (of_int 6)%W8;
+      c <- truncateu16 (t.[2]);
+      c <- c `<<` (of_int 4)%W8;
+      c <- c `|` b;
+      rr.[j] <- (truncateu8 c);
+      (* 
+      Glob.mem <- storeW8 Glob.mem (to_uint (rp + j)) (truncateu8 c); 
+      *)
+      j <- j + 1;
+      b <- truncateu16 (t.[2]);
+      b <- b `>>` (of_int 4)%W8;
+      c <- truncateu16 (t.[3]);
+      c <- c `<<` (of_int 6)%W8;
+      c <- c `|` b;
+      rr.[j] <- (truncateu8 c);
+      (* 
+      Glob.mem <- storeW8 Glob.mem (to_uint (rp + j)) (truncateu8 c); 
+      *)
+      j <- j + 1;
+      t.[3] <- (t.[3]) `>>` (of_int 2)%W8;
+      rr.[j] <- (truncateu8 (t.[3]));
+      (* 
+      Glob.mem <- storeW8 Glob.mem (to_uint (rp + j)) (truncateu8 (t.[3]));
+      *)
+      j <- j + 1;
+    }
+    
+    return rr;
+  }
+
+    proc ref(bp : W16.t Array768.t) : WArray1088.t = {
+       var rr : WArray1088.t;
+       bp <@  Jkem.M(Jkem_avx2.Syscall).__polyvec_reduce(bp);  
+       rr <@ __polyvec_compress_ref(bp);
+       return rr;
+    }
+
+}.
+
+lemma compress10_equiv_avx2mem _ctp _mem :
+   equiv [ AuxPolyVecCompress10.avx2_orig ~  AuxPolyVecCompress10.avx2 :
+      ={bp} /\ ctp{1} = _ctp /\ Glob.mem{1} = _mem /\ valid_ptr (to_uint ctp{1}) (128 + 3 * 320) ==> 
+         Glob.mem{1} = stores _mem (to_uint _ctp) (to_list res{2}) ].
+ admitted.
+
+
+lemma compress10_equiv_refmem _ctp _mem :
+   equiv [ AuxPolyVecCompress10.ref ~  AuxPolyVecCompress10.ref_orig :
+      ={bp} /\ ctp{2} = _ctp /\ Glob.mem{2} = _mem /\ valid_ptr (to_uint ctp{2}) (128 + 3 * 320) ==> 
+         Glob.mem{2} = stores _mem (to_uint _ctp) (to_list res{1}) ].
+ admitted.
+
+(* MAP REDUCE GOAL *)
+lemma compress10_mr : 
+  equiv [AuxPolyVecCompress10.avx2 ~ AuxPolyVecCompress10.ref : lift_array768 bp{1} = lift_array768 bp{2}==> ={res}].
+admitted.
+
+lemma compress10_equiv :
+   equiv [ AuxPolyVecCompress10.avx2_orig ~  AuxPolyVecCompress10.ref_orig :
+      lift_array768 bp{1} = lift_array768 bp{2} /\ valid_ptr (to_uint ctp{1}) (128 + 3 * 320) /\ ={ctp,Glob.mem} ==>  ={Glob.mem}].
+proof. 
+proc* => /=.
+exlim  Glob.mem{1}, ctp{1} => _mem _ctp.
+transitivity {1} { r <@ AuxPolyVecCompress10.avx2(bp); } 
+      (={bp} /\ ctp{1} = _ctp /\ Glob.mem{1} = _mem /\ valid_ptr (to_uint ctp{1}) (128 + 3 * 320) ==> 
+         Glob.mem{1} = stores _mem (to_uint _ctp) (to_list r{2}))
+      (lift_array768 bp{1} = lift_array768 bp{2} /\ ctp{2} = _ctp /\ Glob.mem{2} = _mem /\ valid_ptr (to_uint ctp{2}) (128 + 3 * 320) ==>  Glob.mem{2} = stores _mem (to_uint _ctp) (to_list r{1}));
+   [ by smt() | by smt() | by call (compress10_equiv_avx2mem _ctp _mem); auto => /> |].
+transitivity {2} { r <@ AuxPolyVecCompress10.ref(bp); } 
+    (lift_array768 bp{1} = lift_array768 bp{2} ==> ={r})
+      (={bp} /\ ctp{2} = _ctp /\ Glob.mem{2} = _mem /\ valid_ptr (to_uint ctp{2}) (128 + 3 * 320) ==>  Glob.mem{2} = stores _mem (to_uint _ctp) (to_list r{1}));
+   [ by smt() | by smt() | |  by call (compress10_equiv_refmem _ctp _mem); auto => />].
+by call compress10_mr; auto => />.
+qed.
+
 lemma mlkem_correct_enc_0_avx2 mem _ctp _pkp : 
    equiv [Jkem_avx2.M(Jkem_avx2.Syscall).__indcpa_enc_0 ~ InnerPKE.enc_derand: 
      valid_ptr _pkp (384*3 + 32) /\
@@ -1328,8 +1512,16 @@ seq 47 56 : (={ctp,Glob.mem} /\
     valid_ptr (to_uint ctp{1}) (128+3*320)); last first. 
 wp; conseq (: _ ==> ={Glob.mem}).
 + auto => /> &1 &2 *; do split;1,2:
-    smt (W64.to_uintD_small W64.of_uintK W64.to_uint_cmp pow2_64).
-  admit. (* MAP REDUCE PROOF GOAL *)
+    smt (W64.to_uintD_small W64.of_uintK W64.to_uint_cmp pow2_64). 
+  transitivity {1} { AuxPolyVecCompress10.avx2_orig(ctp,bp); }
+    (={bp,ctp,Glob.mem} ==> ={Glob.mem})
+    ( lift_array768 bp{1} = lift_array768 bp{2} /\ valid_ptr (to_uint ctp{1}) (128 + 3 * 320)  /\ ={ctp,Glob.mem} ==> ={Glob.mem});
+      [ smt() | smt() | by inline*;sim |].
+  transitivity {2} { AuxPolyVecCompress10.ref_orig(ctp,bp); }
+    ( lift_array768 bp{1} = lift_array768 bp{2} /\ valid_ptr (to_uint ctp{1}) (128 + 3 * 320)  /\ ={ctp,Glob.mem} ==> ={Glob.mem})
+    (={bp,ctp,Glob.mem} ==> ={Glob.mem});
+      [ smt() | smt() |  | by inline *;sim].
+  by call compress10_equiv;auto => />.
 
 wp;conseq />.
 call (reduceequiv_noperm).
@@ -1707,8 +1899,20 @@ seq 46  58 : (={ctp0,Glob.mem} /\ Glob.mem{1} = mem /\
     lift_array256 v{1} = lift_array256 v{2} /\ 
     lift_array768 bp{1} = lift_array768 bp{2}); last first. 
 + wp; conseq />; conseq (: _ ==> aux_4{1} = aux_0{2}); 1: by smt().
-  admit. (* MAP REDUCE GOAL *)
-
+  admit.
+(*
++ auto => /> &1 &2 *; do split;1,2:
+    smt (W64.to_uintD_small W64.of_uintK W64.to_uint_cmp pow2_64). 
+  transitivity {1} { AuxPolyVecCompress10.avx2_orig(ctp,bp); }
+    (={bp,ctp,Glob.mem} ==> ={Glob.mem})
+    ( lift_array768 bp{1} = lift_array768 bp{2} /\ valid_ptr (to_uint ctp{1}) (128 + 3 * 320)  /\ ={ctp,Glob.mem} ==> ={Glob.mem});
+      [ smt() | smt() | by inline*;sim |].
+  transitivity {2} { AuxPolyVecCompress10.ref_orig(ctp,bp); }
+    ( lift_array768 bp{1} = lift_array768 bp{2} /\ valid_ptr (to_uint ctp{1}) (128 + 3 * 320)  /\ ={ctp,Glob.mem} ==> ={Glob.mem})
+    (={bp,ctp,Glob.mem} ==> ={Glob.mem});
+      [ smt() | smt() |  | by inline *;sim].
+  by call compress10_equiv;auto => />.
+*)
 wp;conseq />.
 call (reduceequiv_noperm).
 call (addequiv_noperm 4 2 _ _) => //.
